theories/Logic/Syntax.v
@@ -1,0 +1,49 @@
+From CTree Require Import
+                   Events.Core
+                   Logic.Kripke
+                   Utils.Utils.
+
+Generalizable All Variables.
+
+Variant ctlQ := Q_A | Q_E.
+
+Inductive CProp (T: Type): Type :=
+| CBase: T -> CProp T
+| CAnd: CProp T -> CProp T -> CProp T
+| COr: CProp T -> CProp T -> CProp T
+| CImpl: CProp T -> CProp T -> CProp T.
+  
+Section CtlSyntax.
+  Context (E: Type) {HE: Encode E}.
+
+  Inductive ctll :=
+  | CNowL (φ: World E -> Prop): ctll
+  | CgL (q: ctlQ) (φ: ctll): ctll
+  | CxL (q: ctlQ) (φ: ctll): ctll
+  | CuL (q: ctlQ) (φ ψ: ctll): ctll
+  | CPropL (p: CProp ctll): ctll.
+
+  Inductive ctlr (X: Type) :=
+  | CNowR (φ: World E -> Prop): ctlr X
+  | CDoneR (φ: X -> World E -> Prop): ctlr X
+  | CxR (q: ctlQ) (φ: ctlr X): ctlr X
+  | CuR (q: ctlQ) (φ: ctll) (ψ: ctlr X): ctlr X
+  | CPropR (p: CProp (ctlr X)): ctlr X.
+End CtlSyntax.
+
+Arguments CBase {T}.
+Arguments CAnd {T}.
+Arguments COr {T}.
+Arguments CImpl {T}.
+
+Arguments CNowL {E} {HE} φ.
+Arguments CgL {E} {HE} q φ.
+Arguments CxL {E} {HE} q φ.
+Arguments CuL {E} {HE} q φ ψ.
+Arguments CPropL {E} {HE} p.
+
+Arguments CNowR {E} {HE} {X} φ.
+Arguments CDoneR {E} {HE} {X} φ.
+Arguments CxR {E} {HE} {X} q φ.
+Arguments CuR {E} {HE} {X} q φ ψ.
+Arguments CPropR {E} {HE} {X} p.
